working on cancelation & unification.

src/ExprUnify2.v
@@ -7,12 +7,7 @@ Require Import GenRec.
 Set Implicit Arguments.
 Set Strict Implicit.
 
-(** TODO:
- ** this seems like a more difficult interface, but it seems realistic given 
- ** that you can't actually conclude more information after a substitution occurs
- ** you can only ensure that the substitution is consistent with the equation
- **)
-Module Type Unifier.
+Module Type SynUnifier.
   (** An environment that maintains a mapping from variables to their meaning **)
   Parameter Subst : list type -> Type.
 
@@ -21,9 +16,15 @@ Module Type Unifier.
     
     Parameter Subst_empty : Subst types.
 
-    (** The invariant that the substitution implies.
-     **)
-    Parameter SubstInv : forall (funcs : functions types) (meta_env var_env : env types), Subst types -> list (tvar * expr types * expr types) -> Prop.
+    (** Relations **)
+    Parameter Subst_Equal : Subst types -> Subst types -> Prop.
+    Parameter Equiv_Subst_Equal : RelationClasses.Equivalence Subst_Equal.
+
+    Parameter Subst_Le : Subst types -> Subst types -> Prop.
+
+    Parameter Refl_Subst_Le : RelationClasses.Reflexive Subst_Le.
+    Parameter Antisym_Subst_Le : @RelationClasses.Antisymmetric _ _ Equiv_Subst_Equal Subst_Le.
+    Parameter Trans_Subst_Le : RelationClasses.Transitive Subst_Le.
 
     (** The actual unification algorithm **)
     Parameter exprUnify : nat -> expr types -> expr types -> Subst types -> option (Subst types).
@@ -31,44 +32,18 @@ Module Type Unifier.
     (** Substitute meta variables **)
     Parameter exprInstantiate : Subst types -> expr types -> expr types.
 
-    Variable funcs : functions types.
-    Variable vars : env types.
-    
-    (** NOTE: the meaning of Prop isn't quite perfect. We currently reflect Props
-     ** but we actually mean proofs, i.e. using the Provable predicate.
-     **)
-    Definition unifies uenv env (t : tvar) (l r : expr types) : Prop :=
-      match exprD funcs uenv env l t , exprD funcs uenv env r t with
-        | Some l , Some r => match t as t return tvarD types t -> tvarD types t -> Prop with
-                               | tvProp => fun l r => l <-> r (** we'll weaken things a bit more **)
-                               | tvType _ => fun l r => l = r
-                             end l r
-        | _ , _ => False
-      end.
-
-    Axiom SubstInv_empty : forall uenv env sub,
-      SubstInv funcs uenv env sub nil.
-
-    Axiom SubstInvD : forall uenv env sub ctx,
-      SubstInv funcs uenv env sub ctx ->
-      Forall (fun t_l_r => 
-        let '(t,l,r) := t_l_r in
-        unifies uenv env t l r) ctx.
-
     (** This is the soundness statement.
-     ** TODO: Is this correct?
      **)
-    Axiom exprUnify_sound : forall env uenv l r t sub sub' n ctx,
+    Axiom exprUnify_sound : forall n l r sub sub',
       exprUnify n l r sub = Some sub' ->
-      SubstInv funcs uenv env sub ctx ->
-      is_well_typed funcs uenv env l t = true ->
-      is_well_typed funcs uenv env r t = true ->
-      SubstInv funcs uenv env sub' ((t,l,r) :: ctx).
+      exprInstantiate sub' l = exprInstantiate sub' r.
+
+    Axiom exprUnify_extends : forall n l r sub sub',
+      exprUnify n l r sub = Some sub' ->
+      Subst_Le sub' sub.
 
   End typed.
-
-End Unifier.
-
+End SynUnifier.
 
 Inductive R_expr (ts : list type) : expr ts -> expr ts -> Prop :=
 | R_EqualL : forall t l r, R_expr l (Equal t l r)
@@ -93,288 +68,414 @@ Proof.
   exact  v.
 Defined.
 
-Module SUBST := NatMap.IntMap.
+Module Unifier (E : OrderedType.OrderedType with Definition t := nat) : SynUnifier.
+  Module FM := HintlessFMapAVL.Make E.
+  Module FACTS := HintlessFMapFacts.Facts FM.
+  Module MFACTS := NatMap.MoreFMapFacts FM.
+  Module PROPS := HintlessFMapFacts.Properties FM.
 
-Section typed.
-  Variable types : list type.
+  Section typed.
+    Variable types : list type.
 
-  Definition Subst : Type :=
-    SUBST.t (expr types).
+    Section Mentions.
+      Variable uv : nat.
 
-  Definition Subst_lookup (k : nat) (s : Subst) : option (expr types) :=
-    SUBST.find k s.
+      Fixpoint mentionsU (e : expr types) : bool :=
+        match e with
+          | Const _ _ 
+          | Var _ => false
+          | UVar n => if equiv_dec uv n then true else false
+          | Func _ args =>
+            (fix anyb ls : bool := 
+              match ls with
+                | nil => false
+                | l :: ls => mentionsU l || anyb ls
+              end) args
+          | Equal _ l r => mentionsU l || mentionsU r
+          | Not e => mentionsU e
+        end.
+    End Mentions.
 
-  Section Instantiate.
-    Variable sub : Subst.
+    Section Normalization.
+      Variable ctx : FM.t (expr types).
+            
+      Fixpoint normalized (e : expr types) : bool :=
+        match e with
+          | Var _ 
+          | Const _ _ => true
+          | UVar x => match FM.find x ctx with
+                        | None => true
+                        | Some _ => false
+                      end
+          | Not e => normalized e
+          | Equal _ e1 e2 => (normalized e1) && (normalized e2)
+          | Func _ l =>
+            fold_right (fun x acc => acc && (normalized x)) true l
+        end.
+    End Normalization.
 
-    Fixpoint exprInstantiate (e : expr types) : expr types :=
-      match e with 
-        | Const _ _ 
-        | Var _ => e
-        | UVar n => match Subst_lookup n sub with
-                      | None => e 
-                      | Some v => v
-                    end
-        | Func f args => Func f (map exprInstantiate args)
-        | Equal t l r => Equal t (exprInstantiate l) (exprInstantiate r)
-        | Not e => Not (exprInstantiate e)
-      end.
-  End Instantiate.
+    Definition WellFormed (this : FM.t (expr types)) : Prop :=
+      forall k v,
+        FM.MapsTo k v this -> normalized this v = true.
 
-  Section SubstDenote.
-    Variable funcs : functions types.
-    Variable vars : env types.
-    Variable sub : Subst.
+    Definition Subst : Type :=
+      { this : FM.t (expr types) & WellFormed this }.
 
-    Fixpoint Subst_equations (ls : env types) (cur : nat) : env types -> Prop :=
-      match ls with
-        | nil => fun _ => True
-        | l :: ls =>
-          let P := Subst_equations ls (S cur) in
-          match Subst_lookup cur sub with
-            | None => P
-            | Some v => fun g => 
-              match exprD funcs g vars v (projT1 l) with 
-                | Some v => v = projT2 l
-                | None => False
-              end /\ P g
-          end
-      end.
-  End SubstDenote.
+    Definition subst_empty : FM.t (expr types) := FM.empty _. 
 
-  Definition empty_Subst : Subst :=
-    SUBST.empty _.
-
-  Fixpoint anyb T (F : T -> bool) (ls : list T) : bool :=
-    match ls with
-      | nil => false
-      | l :: ls => F l || anyb F ls 
-    end.
-
-  Section Mentions.
-    Variable uv : nat.
-
-    Fixpoint mentionsU (e : expr types) : bool :=
-      match e with
-        | Const _ _ 
-        | Var _ => false
-        | UVar n => if equiv_dec uv n then true else false
-        | Func _ args =>
-          (fix anyb ls : bool := 
-            match ls with
-              | nil => false
-              | l :: ls => mentionsU l || anyb ls
-            end) args
-        | Equal _ l r => mentionsU l || mentionsU r
-        | Not e => mentionsU e
-      end.
-  End Mentions.
-
-  Definition Subst_replace (k : nat) (v : expr types) (s : Subst) : option Subst :=
-    let v' := exprInstantiate s v in
-    if mentionsU k v' then
-      None
-    else
-      let s := SUBST.add k v' s in
-      let s := SUBST.map (exprInstantiate s) s in
-      SUBST.fold (fun k e acc => 
-        match acc with
-          | None => None
-          | _ => 
-            if mentionsU k e then None else acc
-        end) s (Some s).
-  
-  Definition get_Eq (t : tvar) : forall x y : tvarD types t, option (x = y) :=
-    match t as t return forall x y : tvarD types t, option (x = y) with
-      | tvProp => fun _ _ => None
-      | tvType t => 
-        match nth_error types t as k 
-          return forall x y : match k with
-                                | Some t => Impl t
-                                | None => Empty_set
-                              end, option (x = y)
-          with
-          | None =>
-            fun x _ => 
-              match x with
-              end
-          | Some t => Expr.Eq t
-        end 
-    end.
-
-  Section fold_in.
-    Variable LS : list (expr types).
-    Variable F : forall (l r : expr types), Subst -> In l LS -> option Subst.
-
-    Fixpoint dep_in (ls rs : list (expr types)) (sub : Subst) : (forall l, In l ls -> In l LS) -> option Subst.
-    refine (
-      match ls as ls , rs as rs return (forall l, In l ls -> In l LS) -> option Subst with
-        | nil , nil => fun _ => Some sub
-        | l :: ls , r :: rs => fun pf_trans =>
-          match F l r sub _ with
-            | None => None
-            | Some sub => dep_in ls rs sub (fun ls pf => pf_trans _ _)
-          end
-        | _ , _ => fun _ => None
-      end).
-    Focus 2.
-    refine (or_intror _ pf).
-    refine (pf_trans _ (or_introl _ (refl_equal _))).
+    Theorem WF_subst_empty : WellFormed subst_empty.
+      red; unfold subst_empty; intros. apply FACTS.empty_mapsto_iff in H. exfalso; auto.
     Defined.
 
-    Variable F' : forall (l r : expr types), Subst -> option Subst.
+    Definition Subst_empty : Subst :=
+      @existT _ _ subst_empty WF_subst_empty.
 
-    Fixpoint fold2_option (ls rs : list (expr types)) (sub : Subst) : option Subst :=
-      match ls , rs with
-        | nil , nil => Some sub
-        | l :: ls , r :: rs =>
-          match F' l r sub with
-            | None => None
-            | Some sub => fold2_option ls rs sub
-          end
-        | _ , _ => None
+    Definition subst_lookup (k : nat) (s : FM.t (expr types)) : option (expr types) :=
+      FM.find k s.
+    
+    Definition Subst_lookup k (s : Subst) : option (expr types) :=
+      subst_lookup k (projT1 s).
+
+    Section Instantiate.
+      Variable sub : FM.t (expr types).
+
+      Fixpoint subst_exprInstantiate (e : expr types) : expr types :=
+        match e with 
+          | Const _ _ 
+          | Var _ => e
+          | UVar n => match subst_lookup n sub with
+                        | None => e 
+                        | Some v => v
+                      end
+          | Func f args => Func f (map subst_exprInstantiate args)
+          | Equal t l r => Equal t (subst_exprInstantiate l) (subst_exprInstantiate r)
+          | Not e => Not (subst_exprInstantiate e)
+        end.
+    End Instantiate.
+    
+    Definition exprInstantiate (sub : Subst) := subst_exprInstantiate (projT1 sub).
+
+    Definition Subst_Equal (l r : Subst) : Prop := 
+      forall e, exprInstantiate l e = exprInstantiate r e.
+
+    Definition Subst_Le (l r : Subst) : Prop :=
+      forall k v, FM.MapsTo k v (projT1 r) -> 
+        FM.MapsTo k (exprInstantiate l v) (projT1 l).
+
+    Theorem Equiv_Subst_Equal : RelationClasses.Equivalence Subst_Equal.
+    Proof.
+      constructor; unfold Subst_Equal, FM.Equiv; red; intros; subst; eauto.
+      rewrite H; eauto.
+    Qed.    
+
+    Lemma WellFormed_Canonical : forall s v,
+      normalized s v = true ->
+        subst_exprInstantiate s v = v.
+    Proof.
+      induction v; simpl; auto.
+        { unfold subst_lookup. destruct (FM.find x s); auto; congruence. }          
+        { generalize true at 1. intros. f_equal. generalize dependent l.
+          induction 1; simpl; intros; auto.
+          apply andb_true_iff in H1. intuition. f_equal; eauto. }            
+        { intros. apply andb_true_iff in H; f_equal; firstorder. }
+        { intros; f_equal; auto. }
+    Qed.
+
+    Lemma normalized_Lt' : forall s s' v,
+      normalized (projT1 s) v = true -> 
+      Subst_Le s s' ->
+      normalized (projT1 s') v = true.
+    Proof.
+      induction v; simpl; intros; auto.
+      { revert H. case_eq (FM.find x (projT1 s)); intros; try congruence.
+        apply FACTS.not_find_in_iff in H.
+        cutrewrite (FM.find x (projT1 s') = None); auto.
+        apply FACTS.not_find_in_iff. intro. apply H.
+        destruct H2. eapply H0 in H2. eexists; eauto. }
+      { revert H0; revert H1; generalize true at 1 3; induction H; auto; simpl; intros.
+        apply andb_true_iff in H2. apply andb_true_iff. intuition. }
+      { apply andb_true_iff. apply andb_true_iff in H. intuition. }
+    Qed.
+    
+    Lemma WellFormed_subst : forall x y,
+      Subst_Le x y ->
+      forall t, exprInstantiate x (exprInstantiate y t) = exprInstantiate x t.
+    Proof.
+      induction t; simpl; intros; try solve [ auto | f_equal; intuition ].
+      { unfold subst_lookup.
+        case_eq (FM.find x0 (projT1 y)); intros.
+          cutrewrite (FM.find x0 (projT1 x) = Some (exprInstantiate x e)); auto.
+          eapply FACTS.find_mapsto_iff. unfold Subst_Le in *. eapply H.
+          eapply FACTS.find_mapsto_iff. auto.
+
+          case_eq (FM.find x0 (projT1 x)); intros; simpl; unfold subst_lookup; rewrite H1; auto. }
+      { f_equal. induction H0; simpl; auto.
+        f_equal; auto. }
+    Qed.        
+
+    Lemma normalized_Lt : forall s s' w w' v,
+      normalized s' v = true -> 
+      Subst_Le (@existT _ _ s' w') (@existT _ _ s w) ->
+      normalized s v = true.
+    Proof.
+      intros. change s with (projT1 (@existT _ _ s w)). eapply normalized_Lt'; eauto.
+      simpl. auto.
+    Qed.
+
+    Theorem Refl_Subst_Le : RelationClasses.Reflexive Subst_Le.
+    Proof.
+      red; unfold Subst_Le; intros. destruct x; simpl in *.
+      unfold exprInstantiate in *; simpl in *.
+      rewrite WellFormed_Canonical; auto. eapply w; eauto.
+    Qed.
+
+    Theorem Antisym_Subst_Le : @RelationClasses.Antisymmetric _ _ Equiv_Subst_Equal Subst_Le.
+    Proof.
+      red; unfold Subst_Le, Subst_Equal, FM.Equal; intros; eauto.
+      destruct x; destruct y; unfold exprInstantiate in *; simpl in *.
+      induction e; simpl;
+        repeat match goal with
+                 | [ H : _ |- _ ] => rewrite H
+               end; auto.
+      { unfold subst_lookup.
+        case_eq (FM.find x1 x0); intros.
+          eapply FACTS.find_mapsto_iff in H1. generalize H1. eapply w0 in H1. eapply normalized_Lt in H1.
+            2: instantiate (1 := w). 2: instantiate (1 := w0). 2: unfold Subst_Le; simpl; auto.
+            intros.
+            apply H in H2. rewrite WellFormed_Canonical in H2; eauto.
+            eapply FACTS.find_mapsto_iff in H2. rewrite H2; reflexivity.
+
+          eapply FACTS.not_find_in_iff in H1.
+          assert (~FM.In x1 x).
+          intro. apply H1. apply MFACTS.MapsTo_def.
+          destruct H2. eapply H0 in H2. eauto.
+          apply FACTS.not_find_in_iff in H2. rewrite H2. auto. }
+      { f_equal. induction H1; simpl; f_equal; auto. }
+    Qed.
+
+    Theorem Trans_Subst_Le : RelationClasses.Transitive Subst_Le.
+    Proof.
+      red; unfold Subst_Le; intros.
+        eapply H0 in H1. eapply H in H1.
+        erewrite WellFormed_subst in H1; auto.
+    Qed.
+
+    (** Unification **) 
+    Definition subst_set (k : nat) (v : expr types) (s : FM.t (expr types)) 
+      : option (FM.t (expr types)) :=
+      let v' := subst_exprInstantiate s v in
+      if mentionsU k v'
+      then None
+      else let s := FM.add k v' s in
+           let s := FM.map (subst_exprInstantiate s) s in
+           if FM.fold (fun k e (acc : bool) => if acc then true else mentionsU k e) s false
+           then None
+           else Some s.
+    
+    Lemma subst_set_wf : forall k v s s',
+      WellFormed s ->
+      subst_set k v s = Some s' ->
+      WellFormed s'.
+    Proof.
+      unfold subst_set; intros.
+    Admitted.
+
+    Definition Subst_set (k : nat) (v : expr types) (s : Subst) : option Subst :=
+      match subst_set k v (projT1 s) as t return subst_set k v (projT1 s) = t -> _ with
+        | None => fun _ => None
+        | Some s' => fun pf => Some (@existT _ _ s' (@subst_set_wf _ _ _ _ (projT2 s) pf))
+      end refl_equal.
+    
+    Definition get_Eq (t : tvar) : forall x y : tvarD types t, option (x = y) :=
+      match t as t return forall x y : tvarD types t, option (x = y) with
+        | tvProp => fun _ _ => None
+        | tvType t => 
+          match nth_error types t as k 
+            return forall x y : match k with
+                                  | Some t => Impl t
+                                  | None => Empty_set
+                                end, option (x = y)
+            with
+            | None =>
+              fun x _ => 
+                match x with
+                end
+            | Some t => Expr.Eq t
+          end 
       end.
 
-  End fold_in.
+    Section fold_in.
+      Variable LS : list (expr types).
+      Variable F : forall (l r : expr types), Subst -> In l LS -> option Subst.
 
-  Definition exprUnify_recursor bound_l 
-    (recur : forall a_b, R_pair GenRec.R_nat (@R_expr types) a_b bound_l -> expr types -> Subst -> option Subst)
-    (r : expr types) (sub : Subst) : option Subst.
-  refine (
-        match bound_l as bound_l
-          return (forall a_b, R_pair GenRec.R_nat (@R_expr types) a_b bound_l -> expr types -> Subst -> option Subst)
-          -> option Subst
-          with
-          | (bound,l) =>
-            match l as l , r as r 
-              return (forall a_b, R_pair GenRec.R_nat (@R_expr types) a_b (bound, l) -> expr types -> Subst -> option Subst)
-              -> option Subst
-              with
-              | Const t v , Const t' v' => fun _ =>
-                match equiv_dec t t' with
-                  | left pf => match pf in _ = k return tvarD _ k -> _ with
-                                 | refl_equal => fun v' =>
-                                   if get_Eq t v v'
-                                     then Some sub
-                                     else None
-                               end v'
-                  | right _ => None
+      Fixpoint dep_in (ls rs : list (expr types)) (sub : Subst) : (forall l, In l ls -> In l LS) -> option Subst.
+      refine (
+        match ls as ls , rs as rs return (forall l, In l ls -> In l LS) -> option Subst with
+          | nil , nil => fun _ => Some sub
+          | l :: ls , r :: rs => fun pf_trans =>
+            match F l r sub _ with
+              | None => None
+              | Some sub => dep_in ls rs sub (fun ls pf => pf_trans _ _)
+            end
+          | _ , _ => fun _ => None
+        end).
+        Focus 2.
+        refine (or_intror _ pf).
+        refine (pf_trans _ (or_introl _ (refl_equal _))).
+      Defined.
+ 
+      Variable F' : forall (l r : expr types), Subst -> option Subst.
+
+      Fixpoint fold2_option (ls rs : list (expr types)) (sub : Subst) : option Subst :=
+        match ls , rs with
+          | nil , nil => Some sub
+          | l :: ls , r :: rs =>
+            match F' l r sub with
+              | None => None
+              | Some sub => fold2_option ls rs sub
+            end
+          | _ , _ => None
+        end.
+
+    End fold_in.
+
+    Definition exprUnify_recursor bound_l 
+      (recur : forall a_b, R_pair GenRec.R_nat (@R_expr types) a_b bound_l -> expr types -> Subst -> option Subst)
+      (r : expr types) (sub : Subst) : option Subst.
+    refine (
+      match bound_l as bound_l
+        return (forall a_b, R_pair GenRec.R_nat (@R_expr types) a_b bound_l -> expr types -> Subst -> option Subst)
+        -> option Subst
+        with
+        | (bound,l) =>
+          match l as l , r as r 
+            return (forall a_b, R_pair GenRec.R_nat (@R_expr types) a_b (bound, l) -> expr types -> Subst -> option Subst)
+            -> option Subst
+            with
+            | Const t v , Const t' v' => fun _ =>
+              match equiv_dec t t' with
+                | left pf => match pf in _ = k return tvarD _ k -> _ with
+                               | refl_equal => fun v' =>
+                                 if get_Eq t v v'
+                                   then Some sub
+                                   else None
+                             end v'
+                | right _ => None
+              end
+            | Var v , Var v' => fun _ => 
+              if Peano_dec.eq_nat_dec v v' 
+                then Some sub
+                else None
+            | Func f1 args1 , Func f2 args2 => fun recur =>
+              match equiv_dec f1 f2 with
+                | left _ => 
+                  @dep_in args1 (fun l r s pf => recur (bound, l) _ r s) args1 args2 sub (fun _ pf => pf)
+                | right _ => None
+              end
+            | Equal t1 e1 f1 , Equal t2 e2 f2 => fun recur =>
+              if equiv_dec t1 t2 then
+                match recur (bound, e1) _ e2 sub with
+                  | None => None
+                  | Some sub => recur (bound, f1) _ f2 sub
                 end
-              | Var v , Var v' => fun _ => 
-                if Peano_dec.eq_nat_dec v v' 
-                  then Some sub
-                  else None
-              | Func f1 args1 , Func f2 args2 => fun recur =>
-                match equiv_dec f1 f2 with
-                  | left _ => 
-                    @dep_in args1 (fun l r s pf => recur (bound, l) _ r s) args1 args2 sub (fun _ pf => pf)
-                  | right _ => None
-                end
-              | Equal t1 e1 f1 , Equal t2 e2 f2 => fun recur =>
-                if equiv_dec t1 t2 then
-                  match recur (bound, e1) _ e2 sub with
-                    | None => None
-                    | Some sub => recur (bound, f1) _ f2 sub
+                else
+                  None
+            | Not e1 , Not e2 => fun recur =>
+              recur (bound,e1) _ e2 sub
+            | UVar u , _ =>
+              match Subst_lookup u sub with
+                | None => fun recur =>
+                  Subst_set u r sub
+                | Some l' =>
+                  match bound as bound return 
+                    (forall a_b, R_pair GenRec.R_nat (@R_expr types) a_b (bound,UVar u) -> expr types -> Subst -> option Subst)
+                    -> option Subst with
+                    | 0 => fun _ => None
+                    | S bound => fun recur => recur (bound, l') _ r sub
                   end
-                  else
-                    None
-              | Not e1 , Not e2 => fun recur =>
-                recur (bound,e1) _ e2 sub
-              | UVar u , _ =>
-                match Subst_lookup u sub with
-                  | None => fun recur =>
-                    Subst_replace u r sub
-                  | Some l' =>
-                    match bound as bound return 
-                      (forall a_b, R_pair GenRec.R_nat (@R_expr types) a_b (bound,UVar u) -> expr types -> Subst -> option Subst)
-                      -> option Subst with
-                      | 0 => fun _ => None
-                      | S bound => fun recur => recur (bound, l') _ r sub
-                    end
-                end
-              | l , UVar u =>
-                match Subst_lookup u sub with
-                  | None => fun recur =>
-                    Subst_replace u l sub
-                  | Some r' =>
-                    match bound as bound return 
-                      (forall a_b, R_pair GenRec.R_nat (@R_expr types) a_b (bound,l) -> expr types -> Subst -> option Subst)
-                      -> option Subst with
-                      | 0 => fun _ => None
-                      | S bound => fun recur => recur (bound, l) _ r' sub
-                    end
-                end
-              | _ , _ => fun _ => None
-            end 
-        end recur
-      ); try solve [ apply GenRec.L ; constructor | apply GenRec.R ; constructor; assumption ].
-  Defined.
+              end
+            | l , UVar u =>
+              match Subst_lookup u sub with
+                | None => fun recur =>
+                  Subst_set u l sub
+                | Some r' =>
+                  match bound as bound return 
+                    (forall a_b, R_pair GenRec.R_nat (@R_expr types) a_b (bound,l) -> expr types -> Subst -> option Subst)
+                    -> option Subst with
+                    | 0 => fun _ => None
+                    | S bound => fun recur => recur (bound, l) _ r' sub
+                  end
+              end
+            | _ , _ => fun _ => None
+          end 
+      end recur
+    ); try solve [ apply GenRec.L ; constructor | apply GenRec.R ; constructor; assumption ].
+    Defined.
 
-  (** index by a bound, since the termination argument is not trivial
-   ** it is guaranteed to not make more recursions than the number of
-   ** uvars.
-   **)
-  Definition exprUnify (bound : nat) (l : expr types) : expr types -> Subst -> option Subst :=
-    (@Fix _ _ (guard 4 (GenRec.wf_R_pair GenRec.wf_R_nat (@wf_R_expr types)))
-      (fun _ => expr types -> Subst -> option Subst) exprUnify_recursor) (bound,l).
+    (** index by a bound, since the termination argument is not trivial
+     ** it is guaranteed to not make more recursions than the number of
+     ** uvars.
+     **)
+    Definition exprUnify (bound : nat) (l : expr types) : expr types -> Subst -> option Subst :=
+      (@Fix _ _ (guard 4 (GenRec.wf_R_pair GenRec.wf_R_nat (@wf_R_expr types)))
+        (fun _ => expr types -> Subst -> option Subst) exprUnify_recursor) (bound,l).
 
-  Section equiv.
-    Variable A : Type.
-    Variable R : A -> A -> Prop.
-    Hypothesis Rwf : well_founded R.
-    Variable P : A -> Type.
-    
-    Variable equ : forall x, P x -> P x -> Prop.
-    Hypothesis equ_Equiv : forall x, RelationClasses.Equivalence (@equ x).
+    (** Proofs **)
+    Section equiv.
+      Variable A : Type.
+      Variable R : A -> A -> Prop.
+      Hypothesis Rwf : well_founded R.
+      Variable P : A -> Type.
+      
+      Variable equ : forall x, P x -> P x -> Prop.
+      Hypothesis equ_Equiv : forall x, RelationClasses.Equivalence (@equ x).
+      
+      Variable F : forall x : A, (forall y : A, R y x -> P y) -> P x.
 
-    Variable F : forall x : A, (forall y : A, R y x -> P y) -> P x.
+      Lemma Fix_F_equ : forall (x : A) (r : Acc R x),
+        equ (@F x (fun (y : A) (p : R y x) => Fix_F P F (Acc_inv r p)))
+        (Fix_F P F r).
+      Proof.
+        eapply Acc_inv_dep; intros.
+        simpl in *. reflexivity.
+      Qed.
 
-    Lemma Fix_F_equ : forall (x : A) (r : Acc R x),
-      equ (@F x (fun (y : A) (p : R y x) => Fix_F P F (Acc_inv r p)))
-          (Fix_F P F r).
+      Lemma Fix_F_inv_equ : 
+        (forall (x : A) (f g : forall y : A, R y x -> P y),
+          (forall (y : A) (p : R y x), equ (@f y p) (g y p)) -> equ (@F x f) (@F x g)) ->
+        forall (x : A) (r s : Acc R x), equ (Fix_F P F r) (Fix_F P F s).
+      Proof.
+        intro. intro. induction (Rwf x). intros.
+        erewrite <- Fix_F_equ. symmetry. erewrite <- Fix_F_equ. symmetry.
+        eapply H. intros. eauto.
+      Qed.
+
+    End equiv.
+
+    Lemma Equiv_equiv : Equivalence
+      (fun f g : expr types -> Subst -> option Subst =>
+        forall (a : expr types) (b : Subst), f a b = g a b).
     Proof.
-      eapply Acc_inv_dep; intros.
-      simpl in *. reflexivity.
+      constructor; eauto.
+      red. intros. rewrite H; eauto.
     Qed.
 
-    Lemma Fix_F_inv_equ : 
-       (forall (x : A) (f g : forall y : A, R y x -> P y),
-        (forall (y : A) (p : R y x), equ (@f y p) (g y p)) -> equ (@F x f) (@F x g)) ->
-       forall (x : A) (r s : Acc R x), equ (Fix_F P F r) (Fix_F P F s).
+    Lemma exprUnify_recursor_inv : forall (bound : nat)
+      e1 e2 (sub : Subst) (A B : Acc _ (bound,e1))
+      (w : well_founded (R_pair R_nat (R_expr (ts:=types)))),
+      Fix_F (fun _ : nat * expr types => expr types -> Subst -> option Subst)
+      exprUnify_recursor A e2 sub =
+      Fix_F (fun _ : nat * expr types => expr types -> Subst -> option Subst)
+      exprUnify_recursor B e2 sub.
     Proof.
-      intro. intro. induction (Rwf x). intros.
-      erewrite <- Fix_F_equ. symmetry. erewrite <- Fix_F_equ. symmetry.
-      eapply H. intros. eauto.
-    Qed.
-
-  End equiv.
-
-  Lemma Equiv_equiv : Equivalence
-    (fun f g : expr types -> Subst -> option Subst =>
-      forall (a : expr types) (b : Subst), f a b = g a b).
-  Proof.
-    constructor; eauto.
-    red. intros. rewrite H; eauto.
-  Qed.
-
-
-
-  Lemma exprUnify_recursor_inv : forall (bound : nat)
-    e1 e2 (sub : Subst) (A B : Acc _ (bound,e1))
-    (w : well_founded (R_pair R_nat (R_expr (ts:=types)))),
-    Fix_F (fun _ : nat * expr types => expr types -> Subst -> option Subst)
-    exprUnify_recursor A e2 sub =
-    Fix_F (fun _ : nat * expr types => expr types -> Subst -> option Subst)
-    exprUnify_recursor B e2 sub.
-  Proof.
-    intros.
-    eapply (@Fix_F_inv_equ (nat * expr types) (R_pair R_nat (R_expr (ts:=types)))
-      w
-      (fun _ : nat * expr types => expr types -> Subst -> option Subst)
-      (fun x f g => forall a b, f a b = g a b)
-      (fun _ => Equiv_equiv)
-      exprUnify_recursor).
-    clear. intros.
+      intros.
+      eapply (@Fix_F_inv_equ (nat * expr types) (R_pair R_nat (R_expr (ts:=types)))
+        w
+        (fun _ : nat * expr types => expr types -> Subst -> option Subst)
+        (fun x f g => forall a b, f a b = g a b)
+        (fun _ => Equiv_equiv)
+        exprUnify_recursor).
+      clear. intros.
       unfold exprUnify_recursor. destruct x. destruct e; destruct a; auto;
       repeat match goal with 
                | _ => reflexivity
@@ -400,130 +501,389 @@ Section typed.
       destruct l1; auto. 
       rewrite H. destruct (g (n, a)); auto.
       eapply H0.
-  Qed.
+    Qed.
 
-
-  Theorem exprUnify_unroll : forall bound l r sub,
-    exprUnify bound l r sub = 
-    match l , r with
-      | Const t v , Const t' v' =>
-        match equiv_dec t t' with
-          | left pf => match pf in _ = k return tvarD _ k -> _ with
-                         | refl_equal => fun v' =>
-                           if get_Eq t v v'
-                             then Some sub
-                             else None
-                       end v'
-          | right _ => None
-        end
-      | Var v , Var v' => 
-        if Peano_dec.eq_nat_dec v v' 
-          then Some sub
-          else None
-      | Func f1 args1 , Func f2 args2 =>
-        match equiv_dec f1 f2 with
-          | left _ =>
-            fold2_option (@exprUnify bound) args1 args2 sub
-          | right _ => None
-        end
-      | Equal t1 e1 f1 , Equal t2 e2 f2 =>
-        if equiv_dec t1 t2 then
-          match exprUnify bound e1 e2 sub with
-            | None => None
-            | Some sub => exprUnify bound f1 f2 sub
+    Theorem exprUnify_unroll : forall bound l r sub,
+      exprUnify bound l r sub = 
+      match l , r with
+        | Const t v , Const t' v' =>
+          match equiv_dec t t' with
+            | left pf => match pf in _ = k return tvarD _ k -> _ with
+                           | refl_equal => fun v' =>
+                             if get_Eq t v v'
+                               then Some sub
+                               else None
+                         end v'
+            | right _ => None
           end
-        else
-          None
-      | Not e1, Not e2 =>
-        exprUnify bound e1 e2 sub
-      | UVar u , _ =>
-        match Subst_lookup u sub with
-          | None => Subst_replace u r sub
-          | Some l' =>
-            match bound with
-              | 0 => None
-              | S bound => exprUnify bound l' r sub
+        | Var v , Var v' => 
+          if Peano_dec.eq_nat_dec v v' 
+            then Some sub
+            else None
+        | Func f1 args1 , Func f2 args2 =>
+          match equiv_dec f1 f2 with
+            | left _ =>
+              fold2_option (@exprUnify bound) args1 args2 sub
+            | right _ => None
+          end
+        | Equal t1 e1 f1 , Equal t2 e2 f2 =>
+          if equiv_dec t1 t2 then
+            match exprUnify bound e1 e2 sub with
+              | None => None
+              | Some sub => exprUnify bound f1 f2 sub
             end
-        end
-      | l , UVar u =>
-        match Subst_lookup u sub with
-          | None => Subst_replace u l sub
-          | Some r' =>
-            match bound with
-              | 0 => None
-              | S bound => exprUnify bound l r' sub
-            end
-        end
-      | _ , _ => None
-    end.
-  Proof.
-    intros. unfold exprUnify at 1.
-    match goal with
-      | [ |- context [ guard ?X ?Y ] ] =>
-        generalize (guard X Y)
-    end.
-    intros.    
+            else
+              None
+        | Not e1, Not e2 =>
+          exprUnify bound e1 e2 sub
+        | UVar u , _ =>
+          match Subst_lookup u sub with
+            | None => Subst_set u r sub
+            | Some l' =>
+              match bound with
+                | 0 => None
+                | S bound => exprUnify bound l' r sub
+              end
+          end
+        | l , UVar u =>
+          match Subst_lookup u sub with
+            | None => Subst_set u l sub
+            | Some r' =>
+              match bound with
+                | 0 => None
+                | S bound => exprUnify bound l r' sub
+              end
+          end
+        | _ , _ => None
+      end.
+    Proof.
+      intros. unfold exprUnify at 1.
+      match goal with
+        | [ |- context [ guard ?X ?Y ] ] =>
+          generalize (guard X Y)
+      end.
+      intros. unfold Fix.
+      rewrite <- (@Fix_F_equ (nat * expr types) (R_pair R_nat (R_expr (ts:=types)))
+        (fun _ : nat * expr types => expr types -> Subst -> option Subst)
+        (fun x f g => forall a b, f a b = g a b)
+        (fun _ => Equiv_equiv)
+        exprUnify_recursor
+        (bound,l)
+        (w (bound,l))
+        r sub).
+      destruct l; destruct r; simpl; intros; auto;
+        try solve [
+          repeat match goal with
+                   | [ |- context [ match ?X with 
+                                      | _ => _ 
+                                    end ] ] => destruct X
+                 end; try solve [ auto | 
+                   unfold exprUnify, Fix ;
+                     eapply exprUnify_recursor_inv; eauto ] ].
+      Focus 2.
+      destruct (equiv_dec t t0); auto.
+      unfold exprUnify, Fix.
+      erewrite exprUnify_recursor_inv; eauto.
+      instantiate (1 := (guard 4 (wf_R_pair wf_R_nat (wf_R_expr (ts:=types))) (bound, l1))).
+      match goal with 
+        | [ |- match ?X with 
+                 | _ => _ 
+               end = _ ] => destruct X
+      end; auto.
+      erewrite exprUnify_recursor_inv; eauto.
+
+      match goal with
+        | [ |- match ?X with
+                 | _ => _
+               end = _ ] => destruct X; auto
+      end.
+      generalize (fun (l1 : expr types) (pf : In l1 l) => pf).
+      assert (forall l' l0 sub,
+        forall i : (forall l1 : expr types, In l1 l' -> In l1 l),
+          dep_in l
+          (fun (l1 r0 : expr types) (s : Subst) (pf : In l1 l) =>
+            @Fix_F _ _ (fun _ : nat * expr types => expr types -> Subst -> option Subst)
+            exprUnify_recursor (bound, l1) (@Acc_inv (nat * expr types)
+              (@R_pair nat (expr types) R_nat (@R_expr types))
+              (bound, @Func types f l) (w (bound, @Func types f l)) 
+              (bound, l1)
+              (@R nat (expr types) R_nat (@R_expr types) bound l1
+                (@Func types f l) (@R_Func types f l l1 pf))) r0 s) l' l0 sub i =
+          fold2_option (exprUnify bound) l' l0 sub).
+      induction l'; simpl; intros; destruct l1; auto.
+      erewrite exprUnify_recursor_inv; eauto.
+      instantiate (1 := (guard 4 (wf_R_pair wf_R_nat (wf_R_expr (ts:=types))) (bound, a))).
+      unfold exprUnify, Fix.
+      match goal with
+        | [ |- match ?X with
+                 | _ => _
+               end = _ ] => destruct X; auto
+      end.
+      eapply H.
+    Qed.
+
+    Lemma Subst_set_Extends : forall k v sub sub',
+      Subst_set k v sub = Some sub' ->
+      Subst_Le sub' sub.
+    Proof.
+      unfold Subst_set; simpl; intros.
+      revert H.
+      match goal with
+        | [ |- context [ eq_refl ?X ] ] => generalize (eq_refl X)
+      end.
+      generalize (subst_set k v (projT1 sub)) at 2 3. intro. 
+      destruct o; intros; try congruence.
+        inversion H; clear H; subst.
+        destruct sub. unfold Subst_Le, exprInstantiate; simpl in *.
+      admit.
+    Qed.
+
+    Lemma fold2_option_exprUnify_Le' : forall b l l0 sub sub',
+      fold2_option (exprUnify b) l l0 sub = Some sub' ->
+      Forall
+      (fun l : expr types =>
+        forall (r : expr types) (sub sub' : Subst),
+          exprUnify b l r sub = Some sub' -> Subst_Le sub' sub) l ->
+      Subst_Le sub' sub.
+    Proof.
+      intros.
+      generalize dependent l0. generalize dependent sub.
+      induction H0; destruct l0; simpl in *; try congruence; intros.
+        inversion H; eapply Refl_Subst_Le.
+
+      revert H1; case_eq (exprUnify b x e sub); try congruence; intros.
+      eapply Trans_Subst_Le; eauto. 
+    Qed.
+
+    Theorem exprUnify_extends : forall n l r sub sub',
+      exprUnify n l r sub = Some sub' ->
+      Subst_Le sub' sub.
+    Proof.
+      induction n; induction l; intros; rewrite exprUnify_unroll in *; destruct r; simpl in *;
+        try solve [ 
+          repeat (congruence || eauto ||
+              solve [ eapply Subst_set_Extends; eauto |
+                      eapply Trans_Subst_Le; eauto |
+                      apply Refl_Subst_Le |
+                  eapply fold2_option_exprUnify_Le'; eauto ] ||
+              match goal with
+                | [ H : Equivalence.equiv _ _ |- _ ] => 
+                  unfold Equivalence.equiv in H; subst
+                | [ H : Some _ = Some _ |- _ ] => inversion H; clear H; subst
+                | [ H : match exprUnify ?A ?B ?C ?D with _ => _ end = _ |- _ ] => 
+                  revert H; case_eq (exprUnify A B C D); intros
+                | [ H : match ?X with _ => _ end = _ |- _ ] => destruct X
+              end) ].
+    Qed.
+
+    Lemma fold2_option_exprUnify_Extends : forall b l l0 sub sub',
+      fold2_option (exprUnify b) l l0 sub = Some sub' ->
+      Subst_Le sub' sub.
+    Proof.
+      induction l; destruct l0; simpl in *; try congruence; intros.
+        inversion H; subst; apply Refl_Subst_Le.
+      revert H; case_eq (exprUnify b a e sub); try congruence; intros.
+      eapply Trans_Subst_Le; eauto using exprUnify_extends.
+    Qed.
+
+    Lemma Subst_lookup_Subst_set : forall k v s s',
+      Subst_set k v s = Some s' ->
+      Subst_lookup k s' = Some (exprInstantiate s v).
+    Proof.
+      unfold Subst_set, Subst_lookup; do 4 intro.
+(*
+      case_eq (mentionsU k (exprInstantiate s v)); try congruence.
+      match goal with
+        | [ |- context [ if ?X then _ else _ ] ] => case_eq X; try congruence
+      end; intros.
+      inversion H1; clear H1; subst.
+      rewrite FACTS.map_o. unfold FACTS.option_map. rewrite FACTS.add_o.
+      destruct (FM.E.eq_dec k k); intros. 2: exfalso; auto.
+      f_equal.
+
+      clear. (** TODO: probably not legit **)
+      induction v; simpl; auto.
+        destruct (Subst_lookup x s); auto.
+*)
+    Admitted.
+
+    Lemma Subst_lookup_Extends : forall sub sub' k v,
+      Subst_lookup k sub = Some v ->
+      Subst_Le sub' sub ->
+      Subst_lookup k sub' = Some (exprInstantiate sub' v).
+    Proof.
+
+(*
+      intro. unfold Subst_lookup, Subst_Le. eapply PROPS.map_induction with (m := sub); simpl; intros.
+        eapply FACTS.find_mapsto_iff in H0. exfalso. eapply H. eauto.
+
+        rewrite H1 in H2. rewrite FACTS.add_o in H2.
+        destruct (FM.E.eq_dec x k). inversion H2; clear H2; subst.
+
+*)
+    Admitted.
 
 
-    unfold Fix.
-    rewrite <- (@Fix_F_equ (nat * expr types) (R_pair R_nat (R_expr (ts:=types)))
-      (fun _ : nat * expr types => expr types -> Subst -> option Subst)
-      (fun x f g => forall a b, f a b = g a b)
-      (fun _ => Equiv_equiv)
-      exprUnify_recursor
-      (bound,l)
-      (w (bound,l))
-      r sub).
-    destruct l; destruct r; simpl; intros; auto;
-      try solve [
-        repeat match goal with
-                 | [ |- context [ match ?X with 
-                                    | _ => _ 
-                                  end ] ] => destruct X
-               end; try solve [ auto | 
-                 unfold exprUnify, Fix ;
-                   eapply exprUnify_recursor_inv; eauto ] ].
-    Focus 2.
-    destruct (equiv_dec t t0); auto.
-    unfold exprUnify, Fix.
-    erewrite exprUnify_recursor_inv; eauto.
-    instantiate (1 := (guard 4 (wf_R_pair wf_R_nat (wf_R_expr (ts:=types))) (bound, l1))).
-    match goal with 
-      | [ |- match ?X with 
-               | _ => _ 
-             end = _ ] => destruct X
-    end; auto.
-    erewrite exprUnify_recursor_inv; eauto.
+    Lemma Subst_set_Subst_lookup : forall k v sub sub',
+      Subst_set k v sub = Some sub' ->
+      Subst_lookup k sub' = Some (exprInstantiate sub' v).
+    Proof.
+(*
+      unfold Subst_set, Subst_lookup; intros.
+      destruct (mentionsU k (exprInstantiate sub v)); try congruence.
+      match goal with
+        | [ H : (if ?X then _ else _) = _ |- _ ] => destruct X; try congruence
+      end.
+      inversion H; clear H; subst.
+      rewrite FACTS.map_o. unfold FACTS.option_map.
+      repeat rewrite FACTS.add_o. destruct (FM.E.eq_dec k k); try solve [ exfalso; eauto ].
+      f_equal.
+      clear. revert k; revert sub. induction v; simpl; intros; auto.
+      
 
-    match goal with
-      | [ |- match ?X with
-               | _ => _
-             end = _ ] => destruct X; auto
+
+
+      SearchAbout FM.find.
+
+
+      assert (sub' = FM.map (exprInstantiate (FM.add k (exprInstantiate sub v) sub))
+        (FM.add k (exprInstantiate sub v) sub)).
+      generalize dependent sub'.
+      generalize dependent ((FM.map (exprInstantiate (FM.add k (exprInstantiate sub v) sub))
+           (FM.add k (exprInstantiate sub v) sub))). clear.
+      intro. eapply PROPS.fold_rec with (m := t); intros.
+        inversion H0; clear H0; subst.
+*)
+    Admitted.
+
+
+    Lemma exprInstantiate_extends : forall l r sub sub',
+      exprInstantiate sub l = exprInstantiate sub r ->
+      Subst_Le sub' sub -> 
+      exprInstantiate sub' l = exprInstantiate sub' r.
+    Proof.
+    Admitted.
+
+    Lemma fold2_option_map_sound' : forall (n : nat) (l l0 : list (expr types)) (sub sub' : Subst),
+      fold2_option (exprUnify n) l l0 sub = Some sub' ->
+      Forall
+      (fun l1 : expr types =>
+        forall (r : expr types) (sub0 sub'0 : Subst),
+          exprUnify n l1 r sub0 = Some sub'0 ->
+          exprInstantiate sub'0 l1 = exprInstantiate sub'0 r) l ->
+      map (exprInstantiate sub') l = map (exprInstantiate sub') l0.
+    Proof.
+      intros.
+      generalize dependent l0. revert sub; revert sub'. 
+      induction H0; simpl in *; intros; destruct l0; simpl in *; try congruence; auto.
+      revert H1. case_eq (exprUnify n x e sub); intros; try congruence.
+      f_equal; eauto using exprInstantiate_extends, exprUnify_extends, fold2_option_exprUnify_Extends.
+    Qed.
+
+    Theorem exprUnify_sound : forall n l r sub sub',
+      exprUnify n l r sub = Some sub' ->
+      exprInstantiate sub' l = exprInstantiate sub' r.
+    Proof.
+      induction n; induction l; intros; rewrite exprUnify_unroll in *; destruct r; simpl in *;
+        try solve [ 
+          repeat (congruence || 
+                  solve [ eauto |
+                          eapply exprInstantiate_extends; eauto using exprUnify_extends |
+                          eapply fold2_option_map_sound'; eauto ] ||
+              match goal with
+                | [ H : Equivalence.equiv _ _ |- _ ] => 
+                  unfold Equivalence.equiv in H; subst
+                | [ H : _ |- _ ] => erewrite H by eauto
+                | [ |- _ ] => erewrite Subst_set_Subst_lookup by eauto
+                | [ H : forall (l r : expr types) (sub sub' : Subst), exprUnify _ l r sub = Some sub' -> _ , H' : _ |- _ ] =>
+                  specialize (@H _ _ _ _ H')
+                | [ H : Subst_lookup _ _ = _ |- _ ] =>
+                  eapply Subst_lookup_Extends in H; [ | solve [ eauto using exprUnify_extends ] ]
+                | [ H : match exprUnify ?A ?B ?C ?D with _ => _ end = _ |- _ ] => 
+                  revert H; case_eq (exprUnify A B C D); intros
+                | [ H : match Subst_lookup ?X ?Y with _ => _ end = _ |- _ ] =>
+                  revert H; case_eq (Subst_lookup X Y); intros
+                | [ H : match ?X with _ => _ end = _ |- _ ] => destruct X
+                | [ |- Equal _ _ _ = Equal _ _ _ ] => f_equal
+                | [ |- Func _ _ = Func _ _ ] => f_equal
+              end) ].
+
+repeat (congruence || 
+                  solve [ eauto |
+                          eapply exprInstantiate_extends; eauto using exprUnify_extends |
+                          eapply fold2_option_map_sound'; eauto ] ||
+              match goal with
+                | [ H : Equivalence.equiv _ _ |- _ ] => 
+                  unfold Equivalence.equiv in H; subst
+                | [ H : _ |- _ ] => erewrite H by eauto
+                | [ |- _ ] => erewrite Subst_set_Subst_lookup by eauto
+                | [ H : forall (l r : expr types) (sub sub' : Subst), exprUnify _ l r sub = Some sub' -> _ , H' : _ |- _ ] =>
+                  specialize (@H _ _ _ _ H')
+                | [ H : Subst_lookup _ _ = _ |- _ ] =>
+                  eapply Subst_lookup_Le in H; [ | solve [ eauto using exprUnify_extends ] ]
+                | [ H : match exprUnify ?A ?B ?C ?D with _ => _ end = _ |- _ ] => 
+                  revert H; case_eq (exprUnify A B C D); intros
+                | [ H : match Subst_lookup ?X ?Y with _ => _ end = _ |- _ ] =>
+                  revert H; case_eq (Subst_lookup X Y); intros
+                | [ H : match ?X with _ => _ end = _ |- _ ] => destruct X
+                | [ |- Equal _ _ _ = Equal _ _ _ ] => f_equal
+                | [ |- Func _ _ = Func _ _ ] => f_equal
+              end).
+    Admitted.
+  
+  End typed.
+End Unifier.
+
+(*
+
+Module SUBST := NatMap.IntMap.
+
+Section typed.
+  Variable types : list type.
+
+  Definition Subst : Type :=
+    SUBST.t (expr types).
+
+
+  Definition Subst_lookup (k : nat) (s : Subst) : option (expr types) :=
+    SUBST.find k s.
+
+  
+
+  Section SubstDenote.
+    Variable funcs : functions types.
+    Variable vars : env types.
+    Variable sub : Subst.
+
+
+    Fixpoint Subst_equations (ls : env types) (cur : nat) : env types -> Prop :=
+      match ls with
+        | nil => fun _ => True
+        | l :: ls =>
+          let P := Subst_equations ls (S cur) in
+          match Subst_lookup cur sub with
+            | None => P
+            | Some v => fun g => 
+              match exprD funcs g vars v (projT1 l) with 
+                | Some v => v = projT2 l
+                | None => False
+              end /\ P g
+          end
+      end.
+  End SubstDenote.
+
+  Definition empty_Subst : Subst :=
+    SUBST.empty _.
+
+(*
+  Fixpoint anyb T (F : T -> bool) (ls : list T) : bool :=
+    match ls with
+      | nil => false
+      | l :: ls => F l || anyb F ls 
     end.
-    generalize (fun (l1 : expr types) (pf : In l1 l) => pf).
-    assert (forall l' l0 sub,
-      forall i : (forall l1 : expr types, In l1 l' -> In l1 l),
-      dep_in l
-      (fun (l1 r0 : expr types) (s : Subst) (pf : In l1 l) =>
-        @Fix_F _ _ (fun _ : nat * expr types => expr types -> Subst -> option Subst)
-        exprUnify_recursor (bound, l1) (@Acc_inv (nat * expr types)
-           (@R_pair nat (expr types) R_nat (@R_expr types))
-           (bound, @Func types f l) (w (bound, @Func types f l)) 
-           (bound, l1)
-           (@R nat (expr types) R_nat (@R_expr types) bound l1
-              (@Func types f l) (@R_Func types f l l1 pf))) r0 s) l' l0 sub i =
-      fold2_option (exprUnify bound) l' l0 sub).
-    induction l'; simpl; intros; destruct l1; auto.
-    erewrite exprUnify_recursor_inv; eauto.
-    instantiate (1 := (guard 4 (wf_R_pair wf_R_nat (wf_R_expr (ts:=types))) (bound, a))).
-    unfold exprUnify, Fix.
-    match goal with
-      | [ |- match ?X with
-               | _ => _
-             end = _ ] => destruct X; auto
-    end.
-    eapply H.
-  Qed.
+*)
+
+
 
   (** Syntactic Unification **)
   Section Unifies.
@@ -607,7 +967,7 @@ Module TEST.
   Definition uvars := tvType 0 :: tvType 0 :: tvType 0 :: nil.
   Definition subst := 
     let s := empty_Subst types in
-    Subst_replace 1 (UVar 0) s.
+    Subst_set 1 (UVar 0) s.
   Definition funcs : functions types := nil.
 
   Goal 
@@ -623,3 +983,69 @@ Module TEST.
     compute.
   Abort.
 End TEST.
+*)
+
+
+(**
+(** TODO:
+ ** this seems like a more difficult interface, but it seems realistic given 
+ ** that you can't actually conclude more information after a substitution occurs
+ ** you can only ensure that the substitution is consistent with the equation
+ **)
+Module Type SemUnifier.
+  (** An environment that maintains a mapping from variables to their meaning **)
+  Parameter Subst : list type -> Type.
+
+  Section typed.
+    Variable types : list type.
+    
+    Parameter Subst_empty : Subst types.
+
+    (** The invariant that the substitution implies.
+     **)
+    Parameter SubstInv : forall (funcs : functions types) (meta_env var_env : env types), Subst types -> list (tvar * expr types * expr types) -> Prop.
+
+    (** The actual unification algorithm **)
+    Parameter exprUnify : nat -> expr types -> expr types -> Subst types -> option (Subst types).
+    
+    (** Substitute meta variables **)
+    Parameter exprInstantiate : Subst types -> expr types -> expr types.
+
+    Variable funcs : functions types.
+    Variable vars : env types.
+    
+    (** NOTE: the meaning of Prop isn't quite perfect. We currently reflect Props
+     ** but we actually mean proofs, i.e. using the Provable predicate.
+     **)
+    Definition unifies uenv env (t : tvar) (l r : expr types) : Prop :=
+      match exprD funcs uenv env l t , exprD funcs uenv env r t with
+        | Some l , Some r => match t as t return tvarD types t -> tvarD types t -> Prop with
+                               | tvProp => fun l r => l <-> r (** we'll weaken things a bit more **)
+                               | tvType _ => fun l r => l = r
+                             end l r
+        | _ , _ => False
+      end.
+
+    Axiom SubstInv_empty : forall uenv env sub,
+      SubstInv funcs uenv env sub nil.
+
+    Axiom SubstInvD : forall uenv env sub ctx,
+      SubstInv funcs uenv env sub ctx ->
+      Forall (fun t_l_r => 
+        let '(t,l,r) := t_l_r in
+        unifies uenv env t l r) ctx.
+
+    (** This is the soundness statement.
+     ** TODO: Is this correct?
+     **)
+    Axiom exprUnify_sound : forall env uenv l r t sub sub' n ctx,
+      exprUnify n l r sub = Some sub' ->
+      SubstInv funcs uenv env sub ctx ->
+      is_well_typed funcs uenv env l t = true ->
+      is_well_typed funcs uenv env r t = true ->
+      SubstInv funcs uenv env sub' ((t,l,r) :: ctx).
+
+  End typed.
+
+End Unifier.
+**)
