src/SepCancel.v
@@ -1,0 +1,269 @@
+Require Import List.
+Require Import SepTheoryX PropX.
+Require Import PropXTac.
+Require Import RelationClasses EqdepClass.
+Require Import Expr ExprUnify2.
+Require Import DepList.
+Require Import Setoid.
+Require Import Prover.
+Require Import SepExpr.
+
+Set Implicit Arguments.
+Set Strict Implicit.
+
+Require NatMap Multimap.
+
+Module FM := NatMap.IntMap.
+Module MM := Multimap.Make FM.
+Module MF := NatMap.MoreFMapFacts FM.
+
+Definition BadInj types (e : expr types) := False.
+Definition BadPred (f : func) := False.
+Definition BadPredApply types (f : func) (es : list (expr types)) (_ : env types) := False.
+
+Module SepCancler (SE : SepExprType).
+
+  Section env.
+    Variable types : list type.
+    Variable pcType : tvar.
+    Variable stateType : tvar.
+
+    (** The actual tactic code **)
+    Variable Prover : ProverT types.
+    Variable Prover_correct : ProverT_correct Prover funcs.
+
+    Section fold_left3_opt.
+      Variable T U V A : Type.
+      Variable F : T -> U -> V -> A -> option A.
+
+      Fixpoint fold_left_3_opt (ls : list T) (ls' : list U) (ls'' : list V) 
+        (acc : A) : option A :=
+        match ls, ls', ls'' with 
+          | nil , nil , nil => Some acc
+          | x :: xs , y :: ys , z :: zs => 
+            match F x y z acc with
+              | None => None
+              | Some acc => fold_left_3_opt xs ys zs acc
+            end
+          | _ , _ , _ => None
+        end.
+    End fold_left3_opt.
+
+    Definition unifyArgs (bound : nat) (summ : Facts Prover) (l r : list (expr types)) (ts : list tvar) (sub : Subst types)
+      : option (Subst types) :=
+      fold_left_3_opt 
+        (fun l r t (acc : Subst _) =>
+          if Prove Prover summ (Expr.Equal t l r)
+            then Some acc
+            else exprUnify bound l r acc)
+        l r ts sub.
+
+    Fixpoint unify_remove (bound : nat) (summ : Facts Prover) (l : exprs types) (ts : list tvar) (r : list (exprs types))
+      (sub : Subst types)
+      : option (list (list (expr types)) * Subst types) :=
+        match r with 
+          | nil => None
+          | a :: b => 
+            match unifyArgs bound summ l a ts sub with
+              | None => 
+                match unify_remove bound summ l ts b sub with
+                  | None => None
+                  | Some (x,sub) => Some (a :: x, sub)
+                end
+              | Some sub => Some (b, sub)
+            end
+        end.
+(*
+    Fixpoint unify_remove_all (bound : nat) (summ : Facts Prover) (l r : list (list (expr types))) (ts : list tvar)
+      (sub : Subst types)
+      : list (list (expr types)) * list (list (expr types)) * Subst types :=
+        match l with
+          | nil => (l, r, sub)
+          | a :: b => 
+            match unify_remove bound summ a ts r sub with
+              | None => 
+                let '(l,r,sub) := unify_remove_all bound summ b r ts sub in
+                (a :: l, r, sub)
+              | Some (r, sub) =>
+                unify_remove_all bound summ b r ts sub
+            end
+        end.
+*)
+
+    Require Ordering.
+
+    Definition cancel_list : Type := 
+      list (exprs types * nat).
+
+    (** This function determines whether an expression [l] is more "defined"
+     ** than an expression [r]. An expression is more defined if it "uses UVars later".
+     ** NOTE: This is a "fuzzy property" but correctness doesn't depend on it.
+     **)
+    Fixpoint expr_count_meta (e : expr types) : nat :=
+      match e with
+        | Expr.Const _ _
+        | Var _ => 0
+        | UVar _ => 1
+        | Not l => expr_count_meta l
+        | Equal _ l r => expr_count_meta l + expr_count_meta r
+        | Expr.Func _ args =>
+          fold_left plus (map expr_count_meta args) 0
+      end.
+
+    Definition meta_order_args (l r : exprs types) : Datatypes.comparison :=
+      let cmp l r := Compare_dec.nat_compare (expr_count_meta l) (expr_count_meta r) in
+      Ordering.list_lex_cmp _ cmp l r.
+
+
+    Definition meta_order_funcs (l r : exprs types * nat) : Datatypes.comparison :=
+      match meta_order_args (fst l) (fst r) with
+        | Datatypes.Eq => Compare_dec.nat_compare (snd l) (snd r)
+        | x => x
+      end.
+
+    Definition order_impures (imps : MM.mmap (exprs types)) : cancel_list :=
+      MM.FM.fold (fun k => fold_left (fun (acc : cancel_list) (args : exprs types) => 
+        Ordering.insert_in_order _ meta_order_funcs (args, k) acc)) imps nil.
+
+    Lemma impuresD'_flatten : forall U G cs imps,
+      heq U G cs (impuresD' imps)
+                 (starred' (fun v => Func (snd v) (fst v)) 
+                           (FM.fold (fun f argss acc => 
+                             map (fun args => (args, f)) argss ++ acc) imps nil) Emp).
+    Proof.
+      unfold impuresD'. clear. intros. generalize Emp at 2 3.
+      eapply MM.PROPS.fold_rec; intros.
+        eapply MM.PROPS.fold_Empty; eauto with typeclass_instances.
+
+        rewrite MM.PROPS.fold_Add; eauto with typeclass_instances hprop.
+        rewrite starred'_app. symmetry. rewrite <- starred'_base.
+        rewrite H2.
+        eapply heq_star_frame; try reflexivity. clear.
+        induction e; simpl; intros; try reflexivity.
+        rewrite IHe. reflexivity.
+    Qed.
+
+    Lemma starred'_perm : forall T L R,
+      Permutation.Permutation L R ->
+      forall (F : T -> _) U G cs base,
+      heq U G cs (starred' F L base) (starred' F R base).
+    Proof.
+      clear. induction 1; simpl; intros;
+      repeat match goal with
+               | [ H : _ |- _ ] => rewrite H
+             end; try reflexivity; heq_canceler.
+    Qed.
+
+    Lemma fold_Permutation : forall imps L R,
+      Permutation.Permutation L R ->
+      Permutation.Permutation
+      (FM.fold (fun (f : FM.key) (argss : list (exprs types)) (acc : list (exprs types * FM.key)) =>
+        map (fun args : exprs types => (args, f)) argss ++ acc) imps L)
+      (MM.FM.fold
+        (fun k : MM.FM.key =>
+         fold_left
+           (fun (acc : cancel_list) (args : exprs types) =>
+            Ordering.insert_in_order (exprs types * nat) meta_order_funcs
+              (args, k) acc)) imps R).
+    Proof.
+      clear. intros.
+      eapply @MM.PROPS.fold_rel; simpl; intros; auto.
+        revert H1; clear. revert a; revert b; induction e; simpl; intros; auto.
+        rewrite <- IHe; eauto.
+        
+        destruct (@Ordering.insert_in_order_inserts (exprs types * nat) meta_order_funcs (a,k) b) as [ ? [ ? [ ? ? ] ] ].
+        subst. rewrite H.
+        rewrite <- app_ass.
+        eapply Permutation.Permutation_cons_app.
+        rewrite app_ass. eapply Permutation.Permutation_app; eauto.
+    Qed.
+
+    Lemma order_impures_D : forall U G cs imps,
+      heq U G cs (impuresD' imps)
+                 (starred' (fun v => (Func (snd v) (fst v))) (order_impures imps) Emp).
+    Proof.
+      clear. intros. rewrite impuresD'_flatten. unfold order_impures.
+      eapply starred'_perm. eapply fold_Permutation. reflexivity.
+    Qed.
+    
+    (** NOTE : l and r are reversed here **)
+    Fixpoint cancel_in_order (bound : nat) (summ : Facts Prover) 
+      (ls : cancel_list) (acc rem : MM.mmap (exprs types)) (sub : Subst types) 
+      : MM.mmap (exprs types) * MM.mmap (exprs types) * Subst types :=
+      match ls with
+        | nil => (acc, rem, sub)
+        | (args,f) :: ls => 
+          match MM.FM.find f rem with
+            | None => cancel_in_order bound summ ls (MM.mmap_add f args acc) rem sub
+            | Some argss =>
+              match nth_error sfuncs f with
+                | None => cancel_in_order bound summ ls (MM.mmap_add f args acc) rem sub (** Unused! **)
+                | Some ts => 
+                  match unify_remove bound summ args (SDomain ts) argss sub with
+                    | None => cancel_in_order bound summ ls (MM.mmap_add f args acc) rem sub
+                    | Some (rem', sub) =>
+                      cancel_in_order bound summ ls acc (MM.FM.add f rem' rem) sub
+                  end
+              end                      
+          end
+      end.
+
+    Lemma cancel_in_orderOk : forall U G cs bound summ ls acc rem sub L R S,
+      cancel_in_order bound summ ls acc rem sub = (L, R, S) ->
+      himp U G cs (impuresD' R) (impuresD' L) ->
+      himp U G cs (impuresD' acc) (Star (starred' (fun v => (Func (snd v) (fst v))) ls Emp)
+                                        (impuresD' acc)).
+    Proof.
+      
+    Admitted.
+
+
+    Definition sepCancel (bound : nat) (summ : Facts Prover) (l r : SHeap) :
+      SHeap * SHeap * Subst types :=
+      let ordered_r := order_impures (impures r) in
+      let sorted_l := MM.FM.map (fun v => Ordering.sort _ meta_order_args v) (impures l) in 
+      let '(rf, lf, sub) := 
+        cancel_in_order bound summ ordered_r (MM.empty _) sorted_l (empty_Subst _)
+      in
+      ({| impures := lf ; pures := pures l ; other := other l |},
+       {| impures := rf ; pures := pures r ; other := other r |},
+       sub).
+
+    Theorem sepCancel_correct : forall U G cs bound summ l r l' r' sub ,
+      Valid Prover_correct U G summ ->
+      sepCancel bound summ l r = (l', r', sub) ->
+      himp U G cs (sheapD l) (sheapD r) ->
+      himp U G cs (sheapD l') (sheapD r').
+    Proof.
+      clear. destruct l; destruct r. unfold sepCancel. simpl.
+      intros. repeat rewrite sheapD_sheapD'. repeat rewrite sheapD_sheapD' in H1.
+      destruct l'; destruct r'. unfold sheapD' in *. simpl in *.
+
+      
+    Admitted.
+
+  End env.
+
+  Implicit Arguments Emp [ types pcType stateType ].
+  Implicit Arguments Star [ types pcType stateType ].
+  Implicit Arguments Exists [ types pcType stateType ].
+  Implicit Arguments Func [ types pcType stateType ].
+  Implicit Arguments Const [ types pcType stateType ].
+  Implicit Arguments Inj [ types pcType stateType ].
+
+
+  Lemma change_ST_himp_himp : forall (types : list type)
+    (funcs : functions types) (pc st : tvar)
+    (sfuncs : list (ssignature types pc st))
+    EG G
+    (cs : codeSpec (tvarD types pc) (tvarD types st))
+    (L R : sexpr types pc st),
+    himp funcs sfuncs EG G cs L R ->
+    ST.himp cs
+      (@sexprD types pc st funcs sfuncs EG G L)
+      (@sexprD types pc st funcs sfuncs EG G R).
+  Proof.
+    unfold himp. intros. auto.
+  Qed.
+
+End Make.
